pcuic/theories/PCUICInduction.v
@@ -63,3 +63,4 @@ Proof.
   destruct m; constructor; [|apply auxm].
   split; apply auxt.
 Defined.
+
